fully general tuple-based Urban-style rule induction

thys/Urban_Berghofer_Norrish_rule_induction.thy
@@ -17,12 +17,38 @@ datatype 'O sT = Tvar tvar | Sabs vvar "'O sT" | Sop 'O "'O sT list"
 type_synonym 'O sT_tuple = "'O sT list"
 type_synonym 'T T_tuple = "'T list" 
 
+(* Side-conditions, coming with a "side predicate" and a "side tuple": *)
+datatype ('O,'T) scond = Scond (spred: "'T T_tuple \<Rightarrow> bool") (stuple: "'O sT_tuple")
+
  (* Rules are meant to be intepreted on the type 'T, this is why the side-conditions 
-come with predicates on 'T *)
+come with predicates on 'T tuples of specified arities *)
 datatype ('O,'T) rule = Rule 
   (hyps: "'O sT_tuple list") 
-  (side: "('O sT_tuple \<times> ('T T_tuple \<Rightarrow> bool)) list")
+  (side: "('O,'T) scond list")
   (conc: "'O sT_tuple")
+
+
+(* Well-formed schematic terms according to an arity specification *)
+fun wfST :: "('O \<Rightarrow> nat) \<Rightarrow> 'O sT \<Rightarrow> bool" where 
+"wfST ar (Tvar tv) \<longleftrightarrow> True"
+|
+"wfST ar (Sabs vv st) \<longleftrightarrow> wfST ar st"
+|
+"wfST ar (Sop op sts) \<longleftrightarrow> (length sts = ar op) \<and> (\<forall>st \<in> set sts. wfST ar st)"
+
+fun wfST_tuple :: "('O \<Rightarrow> nat) \<Rightarrow> 'O sT_tuple \<Rightarrow> bool" where 
+"wfST_tuple ar sts \<longleftrightarrow> (\<forall>st \<in> set sts. wfST ar st)"
+
+
+(* well-formed rule according to an operation-arity spec "ar" and a number "n": 
+-- they have all tuples well-formed 
+-- have all hypotheses and the conclusion of fixed length n 
+(NB: the side-conditions are allowed any arities)
+*)
+definition wfR where 
+"wfR ar n rl \<equiv> 
+  (\<forall>sts \<in> set (hyps rl) \<union> {conc rl}. wfST_tuple ar sts \<and> length sts = n) \<and> 
+  (\<forall>pred ss. Scond pred ss \<in> set (side rl) \<longrightarrow> wfST_tuple ar ss)"
 
 (* It seems that we do need the "vars" operator from UBN; 
 they do not use it in their result *)
@@ -40,7 +66,7 @@ fun varsbp_tuple :: "'O sT_tuple \<Rightarrow> vvar set" where
 definition varsbpR where 
 "varsbpR rl = 
   (\<Union> (varsbp_tuple ` (set (hyps rl)))) \<union>
-  (\<Union> ((varsbp_tuple o fst) ` (set (side rl)))) \<union>
+  (\<Union> ((varsbp_tuple o stuple) ` (set (side rl)))) \<union>
   varsbp_tuple (conc rl) "
 
 lemma finite_varsbp: "finite (varsbp st)"
@@ -63,6 +89,8 @@ and
 Abs :: "'A \<Rightarrow> 'T \<Rightarrow> 'T" 
 and 
 Op :: "'O \<Rightarrow> 'T list \<Rightarrow> 'T" 
+and 
+arity :: "'O \<Rightarrow> nat"
 assumes  
 Tmap_id: "Tmap id = id"
 and 
@@ -79,11 +107,38 @@ and
 convention from UBN): *)
 Abs_equiv: "\<And>\<sigma> a t. ssbij \<sigma> \<Longrightarrow> Tmap \<sigma> (Abs a t) = Abs (\<sigma> a) (Tmap \<sigma> t)"
 and
-Op_equiv: "\<And>\<sigma> op ts. ssbij \<sigma> \<Longrightarrow> Tmap \<sigma> (Op op ts) = Op op (map (Tmap \<sigma>) ts)"
+Op_equiv: "\<And>\<sigma> op ts. ssbij \<sigma> \<Longrightarrow> length ts = arity op \<Longrightarrow> Tmap \<sigma> (Op op ts) = Op op (map (Tmap \<sigma>) ts)"
 begin
 
-lemma Tmap_comp': "\<And>\<sigma> \<tau> t. ssbij \<sigma> \<Longrightarrow> ssbij \<tau> \<Longrightarrow> Tmap (\<sigma> o \<tau>) t = Tmap \<sigma> (Tmap \<tau> t)"
+lemma Tmap_comp': "ssbij \<sigma> \<Longrightarrow> ssbij \<tau> \<Longrightarrow> Tmap (\<sigma> o \<tau>) t = Tmap \<sigma> (Tmap \<tau> t)"
 using Tmap_comp by fastforce 
+
+(* Extension of the term infrastructure to term-tuples: *)
+(* *) 
+fun Tfvars_tuple :: "'T T_tuple \<Rightarrow> 'A set" where 
+"Tfvars_tuple ts = \<Union> (Tfvars ` (set ts))"
+
+fun Tmap_tuple :: "('A \<Rightarrow> 'A) \<Rightarrow> 'T T_tuple \<Rightarrow> 'T T_tuple" where 
+"Tmap_tuple f ts = map (Tmap f) ts"
+
+lemma Tmap_tuple_id: "Tmap_tuple id = id"
+using Tmap_id by auto
+
+lemma Tmap_tuple_comp: "ssbij \<sigma> \<Longrightarrow> ssbij \<tau> \<Longrightarrow> Tmap_tuple (\<sigma> o \<tau>) = Tmap_tuple \<sigma> o Tmap_tuple \<tau>"
+using Tmap_comp by auto
+
+lemma small_Tfvars_tuple: "small (Tfvars_tuple ts)" 
+by (auto intro: finite_UN_small simp: small_Tfvars)
+
+lemma Tmap_tuple_Tfvars_tuple: 
+"ssbij \<sigma> \<Longrightarrow> Tfvars_tuple (Tmap_tuple \<sigma> ts) \<subseteq> \<sigma> ` (Tfvars_tuple ts)"
+using Tmap_Tfvars by fastforce
+
+lemma Tmap_tuple_cong_id: "ssbij \<sigma> \<Longrightarrow> (\<forall>a\<in>Tfvars_tuple ts. \<sigma> a = a) \<Longrightarrow> Tmap_tuple \<sigma> ts = ts"
+by (simp add: Tmap_cong_id map_idI) 
+
+lemma Tmap_tuple_comp': "ssbij \<sigma> \<Longrightarrow> ssbij \<tau> \<Longrightarrow> Tmap_tuple (\<sigma> o \<tau>) ts = Tmap_tuple \<sigma> (Tmap_tuple \<tau> ts)"
+using Tmap_tuple_comp by fastforce
 
 (* Interpretation of schematic terms: *)
 fun it :: "(vvar \<Rightarrow> 'A) \<Rightarrow> (tvar \<Rightarrow> 'T) \<Rightarrow> 'O sT \<Rightarrow> 'T" where 
@@ -98,67 +153,63 @@ fun it_tuple :: "(vvar \<Rightarrow> 'A) \<Rightarrow> (tvar \<Rightarrow> 'T) \
 
 (* Consequences of the equivariance assumptions: *)
 
-lemma it_Tmap: "ssbij \<sigma> \<Longrightarrow>  Tmap \<sigma> (it vval tval st) = it (\<sigma> \<circ> vval) (Tmap \<sigma> \<circ> tval) st" 
+lemma it_Tmap: "ssbij \<sigma> \<Longrightarrow> wfST arity st \<Longrightarrow> Tmap \<sigma> (it vval tval st) = it (\<sigma> \<circ> vval) (Tmap \<sigma> \<circ> tval) st" 
 apply(induct st, simp_all) 
-using Abs_equiv Op_equiv 
-by (smt (verit) Op_equiv comp_apply list.map_comp map_eq_conv)+
-
-
-(* *) 
-fun Tfvars_tuple :: "'T T_tuple \<Rightarrow> 'A set" where 
-"Tfvars_tuple ts = \<Union> (Tfvars ` (set ts))"
-
-fun Tmap_tuple :: "('A \<Rightarrow> 'A) \<Rightarrow> 'T T_tuple \<Rightarrow> 'T T_tuple" where 
-"Tmap_tuple f ts = map (Tmap f) ts"
-
-lemma Tmap_tuple_comp': "ssbij \<sigma> \<Longrightarrow> ssbij \<tau> \<Longrightarrow> Tmap_tuple (\<sigma> o \<tau>) ts = Tmap_tuple \<sigma> (Tmap_tuple \<tau> ts)"
-using Tmap_comp' by auto
-
-(* *)
+using Abs_equiv apply simp_all
+by (smt (verit) Op_equiv comp_apply length_map list.map_comp map_eq_conv)
 
 lemma it_tuple_Tmap_tuple: "ssbij \<sigma> \<Longrightarrow> 
-Tmap_tuple \<sigma> (it_tuple vval tval st) = it_tuple (\<sigma> \<circ> vval) (Tmap \<sigma> \<circ> tval) st"
+wfST_tuple arity sts \<Longrightarrow> 
+Tmap_tuple \<sigma> (it_tuple vval tval sts) = it_tuple (\<sigma> \<circ> vval) (Tmap \<sigma> \<circ> tval) sts"
 using it_Tmap by auto
 
 end (* locale UBN_Components *)
 
 (* TODO: eventually switch from 'T to "'T list" to better match UBN *)
-locale UBN = UBN_Components dummy Tmap Tfvars Abs Op
+locale UBN = UBN_Components dummy Tmap Tfvars Abs Op arity 
 for dummy :: 'A 
 and Tmap :: "('A \<Rightarrow> 'A) \<Rightarrow> 'T \<Rightarrow> 'T" and Tfvars :: "'T \<Rightarrow> 'A set"
 (* *)
 and Abs :: "'A \<Rightarrow> 'T \<Rightarrow> 'T" and Op :: "'O \<Rightarrow> 'T list \<Rightarrow> 'T" 
+and arity :: "'O \<Rightarrow> nat"
 + 
-fixes rules :: "('O,'T) rule set"
+fixes 
+n :: nat
+and rules :: "('O,'T) rule set"
 assumes
+wfR_rules: 
+"\<And>rl. rl \<in> rules \<Longrightarrow> wfR arity n rl"
+and 
+(* *)
 side_equiv: (* The side-conditions in the rules must be equivariant: *)
-"\<And>rl \<sigma> ss pred. rl \<in> rules \<Longrightarrow> ssbij \<sigma> \<Longrightarrow> 
-    (ss, pred) \<in> set (side rl) \<Longrightarrow> pred (it_tuple vval tval ss) \<Longrightarrow> pred (Tmap_tuple \<sigma> (it_tuple vval tval ss))"
+"\<And>rl \<sigma> pred ss. rl \<in> rules \<Longrightarrow> ssbij \<sigma> \<Longrightarrow> 
+    Scond pred ss \<in> set (side rl) \<Longrightarrow> pred (it_tuple vval tval ss) \<Longrightarrow> 
+    pred (Tmap_tuple \<sigma> (it_tuple vval tval ss))"
 and 
 VCcomp2: (* the second variable-convention compatibility condition from UBN: *)
 "\<And>rl vval tval. rl \<in> rules \<Longrightarrow> 
-   (\<forall>(ss,pred)\<in>set (side rl). pred (it_tuple vval tval ss)) \<Longrightarrow> 
+   (\<forall>pred ss. Scond pred ss \<in> set (side rl) \<longrightarrow> pred (it_tuple vval tval ss)) \<Longrightarrow> 
    vval ` (varsbpR rl) \<inter> Tfvars_tuple (it_tuple vval tval (conc rl)) = {}"
 begin
 
 definition G' where 
-"G' \<equiv> (\<lambda>R t. \<exists>rl vval tval.
-  t = it_tuple vval tval (conc rl) \<and>
+"G' \<equiv> (\<lambda>R ts. \<exists>rl vval tval.
+  ts = it_tuple vval tval (conc rl) \<and>
   rl \<in> rules \<and> 
-  (\<forall>(ss,pred)\<in>set (side rl). pred (it_tuple vval tval ss)) \<and> 
+  (\<forall>pred ss. Scond pred ss \<in> set (side rl) \<longrightarrow> pred (it_tuple vval tval ss)) \<and> 
   (\<forall>ts\<in>set (hyps rl). R (it_tuple vval tval ts)))"
 
 definition G  :: "('T T_tuple \<Rightarrow> bool) \<Rightarrow> 'A list \<Rightarrow> 'T T_tuple \<Rightarrow> bool" where 
-"G \<equiv> (\<lambda>R xs t. \<exists>rl vval tval.
+"G \<equiv> (\<lambda>R xs ts. \<exists>rl vval tval.
   set xs = vval ` (varsbpR rl) \<and> 
-  t = it_tuple vval tval (conc rl) \<and>
+  ts = it_tuple vval tval (conc rl) \<and>
   rl \<in> rules \<and> 
-  (\<forall>(ss,pred)\<in>set (side rl). pred (it_tuple vval tval ss)) \<and> 
+  (\<forall>pred ss. Scond pred ss \<in> set (side rl) \<longrightarrow> pred (it_tuple vval tval ss)) \<and> 
   (\<forall>ts\<in>set (hyps rl). R (it_tuple vval tval ts)))"
 
 lemma ex_comm2: "(\<exists>x y z. P x y z) = (\<exists>y z x . P x y z)" by auto
 
-lemma G'_G: "G' R t = (\<exists>xs. G R xs t)"
+lemma G'_G: "G' R ts = (\<exists>xs. G R xs ts)"
 unfolding G_def G'_def fun_eq_iff apply safe 
   subgoal for rl vval tval
   apply(subst ex_comm2)
@@ -170,7 +221,7 @@ unfolding G_def G'_def fun_eq_iff apply safe
 
 inductive II :: "'T T_tuple \<Rightarrow> bool" where 
 "rl \<in> rules \<Longrightarrow> 
- (\<forall>(ss,pred)\<in>set (side rl). pred (it_tuple vval tval ss)) \<Longrightarrow> 
+ (\<forall>pred ss. Scond pred ss \<in> set (side rl) \<longrightarrow> pred (it_tuple vval tval ss)) \<Longrightarrow> 
  (\<forall>ts\<in>set (hyps rl). II (it_tuple vval tval ts)) \<Longrightarrow>
  II (it_tuple vval tval (conc rl))"
 
@@ -197,21 +248,27 @@ lemma G_mono: "R \<le> R' \<Longrightarrow> G R v t \<Longrightarrow> G R' v t"
 unfolding G_def le_fun_def by auto blast
  
 lemma G_equiv: 
-assumes "ssbij \<sigma>" "G R v t" 
-shows "G (\<lambda>t'. R (Tmap_tuple (inv \<sigma>) t')) (Vmap \<sigma> v) (Tmap_tuple \<sigma> t)"
+assumes "ssbij \<sigma>" "G R v ts" 
+shows "G (\<lambda>t'. R (Tmap_tuple (inv \<sigma>) t')) (Vmap \<sigma> v) (Tmap_tuple \<sigma> ts)"
 using assms unfolding G_def apply safe subgoal for rl vval tval
 apply(rule exI[of _ rl]) apply(rule exI[of _ "\<sigma> o vval"])
 apply(rule exI[of _ "Tmap \<sigma> o tval"]) apply(intro conjI)
   subgoal unfolding Vmap_def by auto
-  subgoal using it_tuple_Tmap_tuple . 
+  subgoal apply(subst it_tuple_Tmap_tuple) using wfR_rules unfolding wfR_def by auto
   subgoal by auto
-  subgoal apply safe subgoal for ss pred
-  unfolding it_tuple_Tmap_tuple[symmetric] apply(rule side_equiv) by auto .
-  subgoal apply safe subgoal for ts unfolding it_tuple_Tmap_tuple[symmetric] 
-  apply(subst Tmap_tuple_comp'[symmetric])
-    subgoal using ssbij_inv by presburger
-    subgoal .
-    subgoal by (simp add: Tmap_id ssbij_invR) . . . .
+  subgoal apply safe subgoal for pred ss
+  apply(subst it_tuple_Tmap_tuple[symmetric])
+    subgoal by auto
+    subgoal using wfR_rules unfolding wfR_def by auto
+    subgoal apply(rule side_equiv) by auto . .  
+  subgoal apply safe subgoal for ts 
+  apply(subst it_tuple_Tmap_tuple[symmetric]) 
+    subgoal by auto
+    subgoal using wfR_rules unfolding wfR_def by auto
+    subgoal apply(subst Tmap_tuple_comp'[symmetric])
+      subgoal using ssbij_inv by presburger
+      subgoal .
+      subgoal by (simp add: Tmap_id ssbij_invR) . . . . .
 
 lemma G_fresh_simple: 
 assumes "G R v ts"
@@ -225,8 +282,9 @@ end (* context UBN *)
 (* The UBN result is subm=sumed by ours: *)
 sublocale UBN < Induct_simple where dummy = dummy and Tmap = Tmap_tuple 
 and Tfvars = Tfvars_tuple and Vmap = Vmap and Vfvars = Vfvars and G = G apply standard
-apply (auto simp: Tmap_id Tmap_comp' small_Tfvars Tmap_Tfvars Tmap_cong_id Vmap_comp 
-   small_Vfvars Vmap_Vfvars G_mono G_equiv G_fresh_simple) sledgehammer
+using small_Tfvars_tuple Tmap_tuple_Tfvars_tuple Tmap_tuple_cong_id 
+small_Vfvars G_equiv G_fresh_simple
+by (auto simp: Tmap_id Tmap_comp' Vmap_comp Vmap_Vfvars G_mono)  
 
 
 
